Move semantic typing of operators to separate file.

theories/sem_typed.v
@@ -1,15 +1,5 @@
 From tutorial_popl20 Require Export sem_type_formers.
 
-(* Typing for operators *)
-Class SemTyUnboxed `{heapG Σ} (A : sem_ty Σ) :=
-  sem_ty_unboxed v : A v -∗ ⌜ val_is_unboxed v ⌝.
-
-Class SemTyUnOp `{heapG Σ} (op : un_op) (A B : sem_ty Σ) :=
-  sem_ty_un_op v : A v -∗ ∃ w, ⌜ un_op_eval op v = Some w ⌝ ∧ B w.
-
-Class SemTyBinOp `{heapG Σ} (op : bin_op) (A1 A2 B : sem_ty Σ) :=
-  sem_ty_bin_op v1 v2 : A1 v1 -∗ A2 v2 -∗ ∃ w, ⌜ bin_op_eval op v1 v2 = Some w ⌝ ∧ B w.
-
 (* The semantic typing judgment *)
 Definition env_sem_typed `{heapG Σ} (Γ : gmap string (sem_ty Σ))
     (vs : gmap string val) : iProp Σ :=
@@ -22,7 +12,7 @@ Instance: Params (@sem_typed) 2 := {}.
 Notation "Γ ⊨ e : A" := (sem_typed Γ e A)
   (at level 100, e at next level, A at level 200).
 
-Section typed_properties.
+Section sem_typed.
   Context `{heapG Σ}.
   Implicit Types A B : sem_ty Σ.
   Implicit Types C : sem_ty Σ → sem_ty Σ.
@@ -61,53 +51,4 @@ Section typed_properties.
 
   Lemma env_sem_typed_empty vs : env_sem_typed ∅ vs -∗ ⌜vs = ∅⌝.
   Proof. by iIntros "?"; iApply big_sepM2_empty_r. Qed.
-
-  (* Unboxed types *)
-  Global Instance sem_ty_unit_unboxed : SemTyUnboxed ().
-  Proof. by iIntros (v ->). Qed.
-  Global Instance sem_ty_bool_unboxed : SemTyUnboxed sem_ty_bool.
-  Proof. iIntros (v). by iDestruct 1 as (b) "->". Qed.
-  Global Instance sem_ty_int_unboxed : SemTyUnboxed sem_ty_int.
-  Proof. iIntros (v). by iDestruct 1 as (i) "->". Qed.
-  Global Instance sem_ty_ref_unboxed A : SemTyUnboxed (ref A).
-  Proof. iIntros (v). by iDestruct 1 as (i ->) "?". Qed.
-
-  (* Operator typing *)
-  Global Instance sem_ty_un_op_int op : SemTyUnOp op sem_ty_int sem_ty_int.
-  Proof. iIntros (?). iDestruct 1 as (i) "->". destruct op; eauto. Qed.
-  Global Instance sem_ty_un_op_bool : SemTyUnOp NegOp sem_ty_bool sem_ty_bool.
-  Proof. iIntros (?). iDestruct 1 as (i) "->". eauto. Qed.
-
-  Global Instance sem_ty_bin_op_eq A : SemTyUnboxed A → SemTyBinOp EqOp A A sem_ty_bool.
-  Proof.
-    iIntros (? v1 v2) "A1 _". rewrite /bin_op_eval /sem_ty_car /=.
-    iDestruct (sem_ty_unboxed with "A1") as %Hunb.
-    rewrite decide_True; last solve_vals_compare_safe.
-    eauto.
-  Qed.
-  Global Instance sem_ty_bin_op_arith op :
-    TCElemOf op [PlusOp; MinusOp; MultOp; QuotOp; RemOp;
-                 AndOp; OrOp; XorOp; ShiftLOp; ShiftROp] →
-    SemTyBinOp op sem_ty_int sem_ty_int sem_ty_int.
-  Proof.
-    iIntros (? v1 v2); iDestruct 1 as (i1) "->"; iDestruct 1 as (i2) "->".
-    repeat match goal with H : TCElemOf _ _ |- _ => inversion_clear H end;
-      rewrite /sem_ty_car /=; eauto.
-  Qed.
-  Global Instance sem_ty_bin_op_compare op :
-    TCElemOf op [LeOp; LtOp] →
-    SemTyBinOp op sem_ty_int sem_ty_int sem_ty_bool.
-  Proof.
-    iIntros (? v1 v2); iDestruct 1 as (i1) "->"; iDestruct 1 as (i2) "->".
-    repeat match goal with H : TCElemOf _ _ |- _ => inversion_clear H end;
-      rewrite /sem_ty_car /=; eauto.
-  Qed.
-  Global Instance sem_ty_bin_op_bool op :
-    TCElemOf op [AndOp; OrOp; XorOp] →
-    SemTyBinOp op sem_ty_bool sem_ty_bool sem_ty_bool.
-  Proof.
-    iIntros (? v1 v2); iDestruct 1 as (i1) "->"; iDestruct 1 as (i2) "->".
-    repeat match goal with H : TCElemOf _ _ |- _ => inversion_clear H end;
-      rewrite /sem_ty_car /=; eauto.
-  Qed.
-End typed_properties.
+End sem_typed.
